Correttezza compilatore v2

MasterThesis/Compiler/Commons.lean
@@ -9,37 +9,36 @@ def eq_states (s : LOOP.State) (t : SCORE.State) : Prop :=
 
 infix:50 "=ₛ" => eq_states
 
-class PLang (α : Type) where
-  idents : α → Finset Ident
-
-def eq_states_idents {α : Type} [PLang α] (s : LOOP.State) (t : SCORE.State) (P : α) : Prop :=
+def eq_states_idents (s : LOOP.State) (t : SCORE.State) (ids : Finset Ident) : Prop :=
   match s, t with
-  | some σ, some τ => ∀ (x : Ident), x ∈ (PLang.idents P) → some ↑(σ x) = (τ x).head?
+  | some σ, some τ => ∀ (x : Ident), x ∈ ids → some ↑(σ x) = (τ x).head?
   | _     , _      => False
 
 notation:50 s:50 "=[" P:50 "]ₛ" t:50 => eq_states_idents s t P
 
-def SCOREcomIdents (P : SCORE.Com) : Finset Ident :=
+namespace SCORE.Com
+
+def ids (P : SCORE.Com) : Finset Ident :=
   match P with
   | SCORE.Com.SKIP    => {}
   | SCORE.Com.CON x   => {x}
   | SCORE.Com.NOC x   => {x}
   | SCORE.Com.DEC x   => {x}
   | SCORE.Com.INC x   => {x}
-  | SCORE.Com.SEQ P Q => SCOREcomIdents P ∪ SCOREcomIdents Q
-  | SCORE.Com.FOR x P => {x} ∪ SCOREcomIdents P
+  | SCORE.Com.SEQ P Q => ids P ∪ ids Q
+  | SCORE.Com.FOR x P => {x} ∪ ids P
 
-instance : PLang SCORE.Com where
-  idents := SCOREcomIdents
+end SCORE.Com
 
-def LOOPcomIdents (P : LOOP.Com) : Finset Ident :=
+namespace LOOP.Com
+
+def ids (P : LOOP.Com) : Finset Ident :=
   match P with
   | LOOP.Com.SKIP    => {}
   | LOOP.Com.ZER x   => {x}
   | LOOP.Com.ASN x y => {x, y}
   | LOOP.Com.INC x   => {x}
-  | LOOP.Com.SEQ P Q => LOOPcomIdents P ∪ LOOPcomIdents Q
-  | LOOP.Com.FOR x P => {x} ∪ LOOPcomIdents P
+  | LOOP.Com.SEQ P Q => ids P ∪ ids Q
+  | LOOP.Com.FOR x P => {x} ∪ ids P
 
-instance : PLang LOOP.Com where
-  idents := LOOPcomIdents
+end LOOP.Com
