MasterThesis/Compiler/Compiler_v2.lean
@@ -5,7 +5,8 @@ def l2s' (ev : Ident) (P : LOOP.Com) : SCORE.Com :=
   match P with
   | LOOP.Com.SKIP    => SCORE.Com.SKIP
   | LOOP.Com.ZER x   => SCORE.Com.CON x
-  | LOOP.Com.ASN x y => SCORE.Com.FOR y (SCORE.Com.INC ev);;
+  | LOOP.Com.ASN x y => SCORE.Com.CON ev;;
+                        SCORE.Com.FOR y (SCORE.Com.INC ev);;
                         SCORE.Com.CON x;;
                         SCORE.Com.FOR ev (SCORE.Com.INC x);;
                         SCORE.Com.FOR x (SCORE.Com.DEC ev)
